code/hash/Hacl.Spec.SHA2.Vec.fsti
@@ -1,2 +1,0 @@
-module Hacl.Spec.SHA2.Vec
-
